\documentclass[../mainfile.tex]{subfiles}

\begin{document}
				
	\subsection{Tabelle wichtiger 1. Ableitungen}
		{\centering
		{\large
		\renewcommand{\arraystretch}{1.3}
		\begin{tabular}{c|c}
			f(x) =		&	f'(x) =                     \\ \hline
			c           &	0                           \\ \hline
			$x^n$ 	    &	$n \cdot x^{n-1}$ 			\\ \hline
			sin x       &	cos x                       \\ \hline
			cos x       &	-sin x                      \\ \hline
			$e^x$		&	$e^x$         				\\ \hline
			$a^x$ 		&	$log(a) \cdot a^x$  		\\ \hline
			log a       &	$\frac{1}{x}$               \\ \hline
			$log_a x$   &	$\frac{1}{log(a) \cdot x}$                 
		\end{tabular}\par
		}		
		}
		\renewcommand{\arraystretch}{1.3}
		
	\subsection{Ableitungsregeln: (!!!)}
	\begin{enumerate}
		{\large\item[i)] Faktorregel:} \\\\
		f(x) = $c \cdot g(x)$	\qquad	$(c \in \mathbb{R})$ \\
		f'(x) = $c \cdot g'(x)$ \\
		Konstanter Faktor darf vorgezogen werden \\
		\underline{Bsp}: \\ 
		f(x) = $2x^2$ \\
		f'(x) = $(2x^2)'$ = $2 \cdot 2x$ = 4x \\\\
		
		{\large\item[ii)] Summenregel:} \\\\
		f(x) = g(x) + h(x) $\Rightarrow$ f'(x)= g'(x) + h'(x) \\
		\underline{Bsp}: \\ 
		f(x) = $x^3+x^2-x-1 \leftarrow$ f√§llt weg ($-1 \cdot x^0 \rightarrow 0 \cdot (-1) \cdot x^{-1}$) \\
		f'(x) = $3x^2+2x-1$	\\\\
		
		{\large\item[iii)] Produktregel:} \\\\ 
		f(x) = g(x) $\cdot$ h(x) $\Rightarrow f'(x)= g'(x) \cdot h(x) + g(x) \cdot h'(x)$ \\
		\underline{Bsp}: \\ 
		f(x) = $x \cdot sin(x)$ \\
		f'(x) = $1 \cdot sin(x) + x \cos(x)$
		
	\end{enumerate}
\end{document}